<h1>Calculating π using Kepler's third law</h1>
<h2>Brief description</h2>
<p>
Today I used the formula a³/T²=G(M+m)/4π² from the Kepler's third law.<br>
Transforming the said equation will yield<br>
π=√(T²G(M+m)/4a³)<br>
where T is the orbital period, G is the <a target="_blank" href="https://en.wikipedia.org/wiki/Gravitational_constant">gravitational constant, and a is the <a target="_blank" href="https://en.wikipedia.org/wiki/Semi-major_and_semi-minor_axes">semi-major axis</a> of the orbit.<br>
<a target="_blank" href="https://codepen.io/MartianLord/pen/VwPPbVz">demo</a>
<a target="_blank" href="https://github.com/martian17/kepler-pi">Github</a>
<a target="_blank" id="github" href="https://github.com/martian17/kepler-pi">Fork me on Github</a>
</p>